casestudy/pmac_verify_hmac.ec
@@ -1,0 +1,127 @@
+require import AllCore IntDiv CoreMap List.
+from Jasmin require import JModel.
+require import Leakage_models.
+
+
+
+theory T.
+clone import ALeakageModel as LeakageModel.
+
+module M = {
+  var leakages : leakages_t
+  
+  proc verify_hmac_jazz (pmac:W64.t, out:W64.t, len:W64.t, pad:W32.t,
+                         maxpad:W32.t, ret:W32.t) : W32.t = {
+    var aux_0: W32.t;
+    var aux: W64.t;
+    
+    var p:W64.t;
+    var temp_64:W64.t;
+    var off:W64.t;
+    var i:W64.t;
+    var j:W64.t;
+    var c:W32.t;
+    var cmask:W32.t;
+    var temp:W32.t;
+    var res_0:W32.t;
+    
+    aux <- out;
+    p <- aux;
+    aux <- (p + len);
+    p <- aux;
+    aux <- (p - (W64.of_int 1));
+    p <- aux;
+    aux <- (zeroextu64 maxpad);
+    temp_64 <- aux;
+    aux <- (p - temp_64);
+    p <- aux;
+    aux <- (p - (W64.of_int 20));
+    p <- aux;
+    aux <- out;
+    off <- aux;
+    aux <- (off - p);
+    off <- aux;
+    aux <- (W64.of_int 0);
+    i <- aux;
+    aux <- (W64.of_int 0);
+    j <- aux;
+    aux_0 <- (maxpad + (W32.of_int 20));
+    maxpad <- aux_0;
+    
+    leakages <- LeakCond(((truncateu32 j) \ult maxpad)) :: LeakAddr([]) :: leakages;
+    
+    while (((truncateu32 j) \ult maxpad)) {
+      leakages <- LeakAddr([LeakageModel.leak_mem ((W64.to_uint (p + j)))]) :: leakages;
+      aux_0 <- (loadW32 Glob.mem (W64.to_uint (p + j)));
+      c <- aux_0;
+      aux <- j;
+      cmask <- (truncateu32 aux);
+      aux_0 <- (cmask - (truncateu32 off));
+      cmask <- aux_0;
+      aux_0 <- (cmask - (W32.of_int 20));
+      cmask <- aux_0;
+      aux_0 <- (cmask `>>` (W8.of_int 31));
+      cmask <- aux_0;
+      aux_0 <- c;
+      temp <- aux_0;
+      aux_0 <- (temp `^` pad);
+      temp <- aux_0;
+      aux_0 <- (invw cmask);
+      cmask <- aux_0;
+      aux_0 <- (temp `&` cmask);
+      temp <- aux_0;
+      aux_0 <- (res_0 `|` temp);
+      res_0 <- aux_0;
+      aux_0 <- (invw cmask);
+      cmask <- aux_0;
+      aux <- off;
+      temp <- (truncateu32 aux);
+      aux_0 <- (temp - (W32.of_int 1));
+      temp <- aux_0;
+      aux_0 <- (temp - (truncateu32 j));
+      temp <- aux_0;
+      aux_0 <- (temp `>>` (W8.of_int 31));
+      temp <- aux_0;
+      aux_0 <- c;
+      temp <- aux_0;
+      leakages <- LeakAddr([LeakageModel.leak_mem ((W64.to_uint (pmac + i)))]) :: leakages;
+      aux_0 <- (temp `^` (loadW32 Glob.mem (W64.to_uint (pmac + i))));
+      temp <- aux_0;
+      aux_0 <- (temp `&` cmask);
+      temp <- aux_0;
+      aux_0 <- (res_0 `|` temp);
+      res_0 <- aux_0;
+      aux <- (i + (W64.of_int 1));
+      i <- aux;
+      aux <- (zeroextu64 cmask);
+      temp_64 <- aux;
+      aux <- (i `&` temp_64);
+      i <- aux;
+      aux <- (j + (W64.of_int 1));
+      j <- aux;
+    leakages <- LeakCond(((truncateu32 j) \ult maxpad)) :: LeakAddr([]) :: leakages;
+    
+    }
+    aux_0 <- (W32.of_int 0);
+    temp <- aux_0;
+    aux_0 <- (temp - res_0);
+    temp <- aux_0;
+    aux_0 <- (temp `>>` (W8.of_int 31));
+    temp <- aux_0;
+    aux_0 <- temp;
+    res_0 <- aux_0;
+    aux_0 <- (W32.of_int 0);
+    temp <- aux_0;
+    aux_0 <- (temp - res_0);
+    temp <- aux_0;
+    aux_0 <- temp;
+    res_0 <- aux_0;
+    aux_0 <- (invw res_0);
+    temp <- aux_0;
+    aux_0 <- (ret `&` (invw res_0));
+    ret <- aux_0;
+    return (ret);
+  }
+}.
+end T.
+
