casestudy/pmac_verify_hmac_proof_BL_CL32.ec
@@ -1,0 +1,37 @@
+require import AllCore IntDiv CoreMap List.
+from Jasmin require import JModel.
+require import Leakage_models.
+require Pmac_verify_hmac.
+import StdOrder.IntOrder Ring.IntID.
+
+clone import Pmac_verify_hmac.T with
+theory LeakageModel <-  LeakageModelCL32.
+
+lemma offset_div_32 (p offset : W64.t) :
+  to_uint p + 32 <= W64.modulus =>
+  32 %| to_uint p =>
+  0 <= to_uint offset < 32 =>
+  to_uint (p + offset) %/ 32  = to_uint p %/ 32.
+proof. move=> /= h1 h2 h3; rewrite W64.to_uintD_small /= 1:/# divzDl 1:// /#. qed.
+
+equiv l_final : M.verify_hmac_jazz ~ M.verify_hmac_jazz :
+={M.leakages, len, pmac, out, maxpad} /\
+  to_uint pmac{2} + 32 <= W64.modulus /\
+  32 %| to_uint pmac{2}
+==> ={M.leakages}.
+proof.
+proc; inline *; auto.
+while (={maxpad, j, p, M.leakages, len, pmac, out, maxpad} /\ to_uint pmac{2} + 32 <= W64.modulus
+        /\ 32 %| to_uint pmac{2}).
+wp; skip=> />.
++ move=> &1 &2 /= hpmac hdiv32 ht. 
+  rewrite /leak_mem /= /leak_mem_CL32 /=. rewrite !offset_div_32.
+  + by apply hpmac.
+  + by apply hdiv32.
+  + have hi : 0 <= to_uint i{1} < 20. + admit. by smt.
+  + by apply hpmac.
+  + by apply hdiv32.
+  + have hi : 0 <= to_uint i{2} < 20. + admit. by smt.
+  by auto.
+wp; skip=> />.
+qed.
